LambdaS5/coq/LjsRulesCorrectCallPrealloc.v
@@ -49,10 +49,31 @@ Implicit Type jlenv : J.lexical_env.
 Lemma red_expr_call_global_is_finite_ok : forall k, th_call_prealloc k J.prealloc_global_is_finite.
 Proof.
     introv Hcinv Hinv Hvrel Hvrels Halo Hcrel Hlred.
+    inverts Hcrel.
     inverts red_exprh Hlred.
+    ljs_apply.
+    ljs_context_invariant_after_apply.
 Admitted.
 
 Lemma red_expr_call_global_is_nan_ok : forall k, th_call_prealloc k J.prealloc_global_is_nan.
 Proof.
 Admitted.
 
+Lemma red_expr_call_number_ok : forall k, th_call_prealloc k J.prealloc_number.
+Proof.
+    introv Hcinv Hinv Hvrel Hvrels Halo Hcrel Hlred.
+    inverts Hcrel.
+    inverts red_exprh Hlred.
+    ljs_apply.
+    ljs_context_invariant_after_apply.
+Admitted.
+
+Lemma red_expr_call_boolean_ok : forall k, th_call_prealloc k J.prealloc_bool.
+Proof.
+    introv Hcinv Hinv Hvrel Hvrels Halo Hcrel Hlred.
+    inverts Hcrel.
+    inverts red_exprh Hlred.
+    ljs_apply.
+    ljs_context_invariant_after_apply.
+    repeat ljs_autoforward.
+Admitted.
